books/centaur/fgl/aig-eval.lisp
@@ -1,0 +1,420 @@
+ ; GL - A Symbolic Simulation Framework for ACL2
+; Copyright (C) 2018 Centaur Technology
+;
+; Contact:
+;   Centaur Technology Formal Verification Group
+;   7600-C N. Capital of Texas Highway, Suite 300, Austin, TX 78731, USA.
+;   http://www.centtech.com/
+;
+; License: (An MIT/X11-style license)
+;
+;   Permission is hereby granted, free of charge, to any person obtaining a
+;   copy of this software and associated documentation files (the "Software"),
+;   to deal in the Software without restriction, including without limitation
+;   the rights to use, copy, modify, merge, publish, distribute, sublicense,
+;   and/or sell copies of the Software, and to permit persons to whom the
+;   Software is furnished to do so, subject to the following conditions:
+;
+;   The above copyright notice and this permission notice shall be included in
+;   all copies or substantial portions of the Software.
+;
+;   THE SOFTWARE IS PROVIDED "AS IS", WITHOUT WARRANTY OF ANY KIND, EXPRESS OR
+;   IMPLIED, INCLUDING BUT NOT LIMITED TO THE WARRANTIES OF MERCHANTABILITY,
+;   FITNESS FOR A PARTICULAR PURPOSE AND NONINFRINGEMENT. IN NO EVENT SHALL THE
+;   AUTHORS OR COPYRIGHT HOLDERS BE LIABLE FOR ANY CLAIM, DAMAGES OR OTHER
+;   LIABILITY, WHETHER IN AN ACTION OF CONTRACT, TORT OR OTHERWISE, ARISING
+;   FROM, OUT OF OR IN CONNECTION WITH THE SOFTWARE OR THE USE OR OTHER
+;   DEALINGS IN THE SOFTWARE.
+;
+; Original author: Sol Swords <sswords@centtech.com>
+
+(in-package "FGL")
+
+(include-book "primitives")
+(include-book "centaur/aignet/from-hons-aig" :dir :system)
+(local (include-book "primitive-lemmas"))
+(local (std::add-default-post-define-hook :fix))
+
+
+
+(def-gl-formula-checks aig-eval-formula-checks
+  (hons-get
+   hons-assoc-equal
+   hons-equal
+   atom
+   eq
+   acl2::aig-env-lookup
+   acl2::aig-atom-p$inline
+   acl2::aig-eval
+   acl2::aig-eval-list))
+
+(local (def-gl-formula-checks-lemmas aig-eval-formula-checks))
+
+
+(def-formula-check-definition-thm atom                    aig-eval-formula-checks)
+(def-formula-check-definition-thm eq                      aig-eval-formula-checks)
+(def-formula-check-definition-thm hons-equal              aig-eval-formula-checks)
+(def-formula-check-definition-thm hons-assoc-equal        aig-eval-formula-checks)
+(def-formula-check-definition-thm hons-get                aig-eval-formula-checks)
+(def-formula-check-definition-thm acl2::aig-atom-p$inline aig-eval-formula-checks)
+(def-formula-check-definition-thm acl2::aig-env-lookup    aig-eval-formula-checks)
+(def-formula-check-definition-thm acl2::aig-eval          aig-eval-formula-checks)
+(def-formula-check-definition-thm acl2::aig-eval-list     aig-eval-formula-checks)
+
+
+(define gl-object-alist-to-varmap ((x gl-object-alist-p)
+                                   (bfrstate bfrstate-p)
+                                   (acc alistp))
+  :guard (and (bfrstate-mode-is :aignet)
+              (bfr-listp (gl-object-alist-bfrlist x)))
+  :returns (mv err varmap)
+  (if (atom x)
+      (mv nil acc)
+    (if (and (mbt (consp (car x)))
+             (acl2::aig-var-p (caar x))
+             (not (hons-get (caar x) acc)))
+        (b* (((mv ok obj) (gobj-syntactic-boolean-fix (cdar x)))
+             ((unless ok)
+              (mv (msg "Bad symbolic value for key: ~x0~%" (caar x)) nil)))
+          (gl-object-alist-to-varmap
+           (cdr x) bfrstate
+           (hons-acons (caar x)
+                       (bfr->aignet-lit (gobj-syntactic-boolean->bool obj) bfrstate)
+                       acc)))
+      (gl-object-alist-to-varmap (cdr x) bfrstate acc)))
+  ///
+  (defthm good-varmap-p-of-gl-object-alist-to-varmap
+    (b* (((mv ?err varmap) (gl-object-alist-to-varmap x (logicman->bfrstate) acc)))
+      (implies (and (bfrstate-mode-is :aignet (logicman->bfrstate))
+                    (lbfr-listp (gl-object-alist-bfrlist x))
+                    (aignet::good-varmap-p acc (logicman->aignet logicman)))
+               (aignet::good-varmap-p varmap (logicman->aignet logicman))))
+    :hints(("Goal" :in-theory (enable aignet::good-varmap-p))))
+
+  ;; (defret lookup-preserved-in-<fn>
+  ;;   (implies (and (not err)
+  ;;                 (equal acc-pair (hons-assoc-equal key acc))
+  ;;                 acc-pair)
+  ;;            (equal (hons-assoc-equal key varmap)
+  ;;                   acc-pair)))
+
+  ;; (defret lookup-exists-in-gl-object-alist-to-varmap
+  ;;   (implies (and (not err)
+  ;;                 (acl2::aig-var-p key)
+  ;;                 (hons-assoc-equal key x))
+  ;;            (hons-assoc-equal key varmap)))
+
+  (defret lookup-exists-in-gl-object-alist-to-varmap-split
+    (implies (not err)
+             (iff (hons-assoc-equal key varmap)
+                  (or (hons-assoc-equal key acc)
+                      (and (acl2::aig-var-p key)
+                           (hons-assoc-equal key x))))))
+  
+  (defret lookup-in-gl-object-alist-to-varmap
+    (implies (and (not err)
+                  (hons-assoc-equal key varmap))
+             (equal (hons-assoc-equal key varmap)
+                    (or (hons-assoc-equal key acc)
+                        (and (acl2::aig-var-p key)
+                             (cons key
+                                   (bfr->aignet-lit (gobj-syntactic-boolean->bool
+                                                     (mv-nth 1 (gobj-syntactic-boolean-fix
+                                                                (cdr (hons-assoc-equal key x)))))
+                                                    bfrstate))))))
+    :hints(("Goal" :in-theory (enable hons-assoc-equal))))
+
+  (defret gobj-syntactic-boolean-fix-when-gl-object-alist-to-varmap
+    (implies (and (not err)
+                  (hons-assoc-equal key varmap)
+                  (not (hons-assoc-equal key acc)))
+             (mv-nth 0 (gobj-syntactic-boolean-fix (cdr (hons-assoc-equal key x)))))))
+
+
+
+(define lit-list-max-var+1 ((x aignet::lit-listp))
+  :returns (max-var natp :rule-classes :type-prescription)
+  (if (atom x)
+      0
+    (max (+ 1 (satlink::lit->var (car x)))
+         (lit-list-max-var+1 (cdr x))))
+  ///
+  (defthm lit-list-max-var+1-when-aignet-lit-listp
+    (implies (aignet::aignet-lit-listp x aignet)
+             (<= (lit-list-max-var+1 x) (+ 1 (aignet::fanin-count aignet))))
+    :hints(("Goal" :in-theory (enable aignet::aignet-idp))))
+
+  (defthm lit-list-max-var+1-of-aiglist-to-aignet
+    (b* (((mv lits & & new-aignet) (aignet::aiglist-to-aignet aigs xmemo varmap gatesimp strash aignet)))
+      (implies (and (aignet::good-varmap-p varmap aignet)
+                    (aignet::xmemo-well-formedp xmemo aignet))
+               (<= (lit-list-max-var+1 lits) (+ 1 (aignet::fanin-count new-aignet)))))
+    :hints (("goal" :use ((:instance lit-list-max-var+1-when-aignet-lit-listp
+                           (x (mv-nth 0 (aignet::aiglist-to-aignet aigs xmemo varmap gatesimp strash aignet)))
+                           (aignet (mv-nth 3 (aignet::aiglist-to-aignet aigs xmemo varmap gatesimp strash aignet)))))
+             :in-theory (disable lit-list-max-var+1-when-aignet-lit-listp
+                                 lit-list-max-var+1)))
+    :rule-classes :linear))
+
+(encapsulate nil
+  (define aignet-lit->bool ((x satlink::litp)
+                            (bfrstate bfrstate-p))
+    :guard (and (bfrstate-mode-is :aignet)
+                (<= (satlink::lit->var x) (bfrstate->bound bfrstate)))
+    :returns (obj gl-object-p)
+    (g-boolean (aignet-lit->bfr x bfrstate))
+    ///
+    (defret bfr-listp-of-aignet-lit->bool
+      (implies (and (bfrstate-mode-is :aignet)
+                    (<= (satlink::lit->var x) (bfrstate->bound bfrstate)))
+               (bfr-listp (gl-object-bfrlist obj))))
+
+    (defret fgl-object-eval-of-<fn>
+      (implies (lbfr-mode-is :aignet)
+               (equal (fgl-object-eval (aignet-lit->bool x (logicman->bfrstate)) env)
+                      (b* ((aignet (logicman->aignet logicman)))
+                        (bit->bool
+                         (aignet::lit-eval x
+                                           (alist-to-bitarr (aignet::num-ins aignet)
+                                                            (gl-env->bfr-vals env) nil)
+                                           ;; (alist-to-bitarr (aignet::num-regs aignet) nil nil)
+                                           nil
+                                           aignet)))))
+      :hints(("Goal" :in-theory (enable gobj-bfr-eval bfr-eval)))))
+  ;; (local (set-default-hints
+  ;;         '((and stable-under-simplificationp
+  ;;                '(:expand ((lit-list-max-var+1 x)))))))
+  (local (in-theory (enable lit-list-max-var+1
+                            satlink::lit-listp)))
+
+  ;; (define gl-objectlist-to-object ((x gl-objectlist-p))
+  ;;   :returns (new-x gl-object-p)
+  ;;   (if (atom x)
+  ;;       nil
+  ;;     (g-cons (car x)
+  ;;             (gl-objectlist-to-object (cdr x))))
+  ;;   ///
+  ;;   (defret fgl-object-eval-of-<fn>
+  ;;     (equal (fgl-object-eval new-x env)
+  ;;            (fgl-objectlist-eval x env)))
+
+  ;;   (defret gl-objectlist-bfrlist-of-<fn>
+  ;;     (implies (not (member v (gl-objectlist-bfrlist x)))
+  ;;              (not (member v (gl-object-bfrlist new-x))))))
+
+  ;; (define gl-objectlist-accumulate-to-object ((x gl-objectlist-p)
+  ;;                                             (acc gl-object-p))
+  ;;   :returns (new-x gl-object-p)
+  ;;   (if (atom x)
+  ;;       (gl-object-fix acc)
+  ;;     (gl-objectlist-accumulate-to-object
+  ;;      (cdr x)
+  ;;      (g-cons (car x) acc)))
+  ;;   )
+
+  ;; (define aignet-lit-list->bools-aux ((x aignet::lit-listp)
+  ;;                                     (bfrstate bfrstate-p)
+  ;;                                     (acc gl-objectlist-p))
+  ;;   :returns (obj gl-object-p)
+  ;;   (if (Atom x)
+  ;;       (gl-objectlist-accumulate-to-object acc nil)
+  ;;     (aignet-lit-list->bools-aux
+  ;;      (cdr x) bfrstate (cons (aignet-lit->bool (car x) bfrstate acc)))))
+
+  (define aignet-lit-list->bools ((x aignet::lit-listp)
+                                  (bfrstate bfrstate-p))
+    :returns (new-x gl-object-p)
+    :guard (and (bfrstate-mode-is :aignet)
+                (<= (lit-list-max-var+1 x) (+ 1 (bfrstate->bound bfrstate))))
+    :guard-debug t
+    ;; :verify-guards nil
+    (if (atom x)
+        nil
+      (mk-g-cons (aignet-lit->bool (car x) bfrstate)
+                 (aignet-lit-list->bools (cdr x) bfrstate)))
+    ///
+    ;; (verify-guards aignet-lit-list->bfrs-nrev
+    ;;   :hints(("Goal" :in-theory (enable lit-list-max-var+1))))
+    ;; (verify-guards aignet-lit-list->bfrs
+    ;;   :hints(("Goal" :in-theory (enable lit-list-max-var+1))))
+    
+    (defthm bfr-listp-of-aignet-lit-list->bools
+      (implies (and (<= (lit-list-max-var+1 x) (+ 1 (bfrstate->bound bfrstate)))
+                    (bfrstate-mode-is :aignet))
+               (bfr-listp (gl-object-bfrlist (aignet-lit-list->bools x bfrstate))))
+      :hints(("Goal" :in-theory (enable aignet-lit-list->bools
+                                        lit-list-max-var+1))))
+    (defthm fgl-object-eval-of-aignet-lit-list->bools
+      (implies (lbfr-mode-is :aignet)
+               (equal (fgl-object-eval (aignet-lit-list->bools x (logicman->bfrstate)) env)
+                      (b* ((aignet (logicman->aignet logicman)))
+                        (bits->bools
+                         (aignet::lit-eval-list x
+                                                (alist-to-bitarr (aignet::num-ins aignet)
+                                                                 (gl-env->bfr-vals env) nil)
+                                                nil
+                                                aignet)))))
+      :hints(("Goal" :in-theory (enable bits->bools))))))
+
+
+(set-ignore-ok t)
+
+(local (defthm good-varmap-p-nil
+         (aignet::good-varmap-p nil aignet)
+         :hints(("Goal" :in-theory (enable aignet::good-varmap-p)))))
+
+;; (local (defthm logicman->bfrstate-of-update-logicman->aignet
+;;          (implies (lbfr-mode-is :aignet)
+;;                   (equal (logicman->bfrstate (update-logicman->aignet aignet logicman))
+;;                          (bfrstate (lbfr-mode)
+;;                                    (aignet::fanin-count aignet))))
+;;          :hints(("Goal" :in-theory (enable logicman->bfrstate)))))
+
+(local (defthm logicman-extension-p-of-update
+         (implies (and (equal (logicman->aignet new) (logicman->aignet old))
+                       (equal (logicman->mode new) (logicman->mode old)))
+                  (logicman-extension-p new old))
+         :hints(("Goal" :in-theory (enable logicman-extension-p)))))
+
+(local (defthm logicman-extension-p-of-update-aignet
+         (implies (and (aignet::aignet-extension-p new-aignet (logicman->aignet old))
+                       (equal (aignet::num-regs new-aignet) (aignet::num-regs (logicman->aignet old))))
+                  (logicman-extension-p (update-logicman->aignet new-aignet old) old))
+         :hints(("Goal" :in-theory (enable logicman-extension-p)))))
+         
+(local (include-book "tools/trivial-ancestors-check" :dir :system))
+(local (acl2::use-trivial-ancestors-check))
+
+(local (defthm fgl-objectlist-eval-when-atom
+         (implies (not (consp x))
+                  (equal (fgl-objectlist-eval x env) nil))
+         :hints(("Goal" :in-theory (enable fgl-objectlist-eval)))
+         :rule-classes ((:rewrite :backchain-limit-lst 0))))
+
+(local (defthm boolean-listp-of-aig-eval-list
+         (boolean-listp (acl2::aig-eval-list x env))))
+
+(local (defthm bits->bools-of-bools->bits
+         (implies (boolean-listp x)
+                  (equal (bits->bools (aignet::bools->bits x)) x))
+         :hints(("Goal" :in-theory (enable aignet::bools->bits bits->bools)))))
+
+(local (defun-sk aig-env-equiv (x y)
+         (forall v
+                 (implies (acl2::aig-var-p v)
+                          (equal (acl2::aig-env-lookup v x)
+                                 (acl2::aig-env-lookup v y))))
+         :rewrite :direct))
+
+(local (defthm aig-env-equiv-self
+         (aig-env-equiv x x)
+         :hints(("Goal" :in-theory (enable aig-env-equiv)))))
+
+(local (defthm aig-env-equiv-symm
+         (implies (aig-env-equiv x y)
+                  (aig-env-equiv y x))
+         :hints(("Goal" :expand ((aig-env-equiv y x))
+                 :in-theory (disable acl2::aig-env-lookup)))))
+
+(local (defthm aig-env-equiv-trans
+         (implies (and (aig-env-equiv x y)
+                       (aig-env-equiv y z))
+                  (aig-env-equiv x z))
+         :hints(("Goal" :expand ((aig-env-equiv x z))
+                 :in-theory (disable acl2::aig-env-lookup)))))
+
+(local (defequiv aig-env-equiv))
+
+(local (in-theory (disable aig-env-equiv
+                           aig-env-equiv-symm
+                           aig-env-equiv-necc)))
+
+;; (local (defcong aig-env-equiv equal (acl2::aig-env-lookup v x) 2
+;;          :hints(("Goal" :in-theory (disable acl2::aig-env-lookup)
+;;                  :use ((:instance aig-env-equiv-necc
+;;                         (y x-equiv)))))))
+
+(local (defcong aig-env-equiv equal (acl2::aig-eval v x) 2
+         :hints(("Goal" :in-theory (disable acl2::aig-env-lookup)
+                 :induct (acl2::aig-eval v x))
+                (and stable-under-simplificationp
+                     '(:use ((:instance aig-env-equiv-necc
+                              (y x-equiv))))))))
+
+(local (defcong aig-env-equiv equal (acl2::aig-eval-list v x) 2
+         :hints(("Goal" :in-theory (disable acl2::aig-env-lookup)))))
+
+(local (defthm lookup-exists-of-fgl-object-alist-eval
+         (iff (hons-assoc-equal k (fgl-object-alist-eval x env))
+              (hons-assoc-equal k x))
+         :hints(("Goal" :in-theory (enable fgl-object-alist-eval hons-assoc-equal)))))
+
+(local (defthm lookup-of-fgl-object-alist-eval
+         (equal (cdr (hons-assoc-equal k (fgl-object-alist-eval x env)))
+                (fgl-object-eval (cdr (hons-assoc-equal k x)) env))
+         :hints(("Goal" :in-theory (enable fgl-object-alist-eval hons-assoc-equal)))))
+
+(local (defthm lit-eval-bfr->aignet-lit-is-bfr-eval
+         (implies (lbfr-mode-is :Aignet)
+                  (equal (aignet::lit-eval
+                          (bfr->aignet-lit x (logicman->bfrstate))
+                          (alist-to-bitarr (aignet::stype-count :pi (logicman->aignet logicman))
+                                           (gl-env->bfr-vals env) nil)
+                          nil
+                          (logicman->aignet logicman))
+                         (bool->bit (gobj-bfr-eval x env))))
+         :hints(("Goal" :in-theory (enable bfr-eval gobj-bfr-eval)))))
+
+
+(local (defthm aig-env-equiv-of-aignet-eval-to-env
+         (b* (((mv err varmap) (GL-OBJECT-ALIST-TO-VARMAP
+                                           alist
+                                           (logicman->bfrstate)
+                                           NIL)))
+           (implies (and (lbfr-mode-is :aignet)
+                         (not err))
+                    (aig-env-equiv (AIGNET::AIGNET-EVAL-TO-ENV
+                                    varmap
+                                    (ALIST-TO-BITARR
+                                     (AIGNET::STYPE-COUNT :PI (logicman->aignet logicman))
+                                     (GL-ENV->BFR-VALS ENV)
+                                     NIL)
+                                    NIL
+                                    (logicman->aignet logicman))
+                                   (fgl-object-alist-eval alist env))))
+         :hints(("Goal" :in-theory (e/d (aig-env-equiv
+                                         lookup-exists-in-gl-object-alist-to-varmap-split))))))
+
+
+
+(def-gl-primitive acl2::aig-eval-list (x a)
+  (gl-object-case x
+    :g-concrete (gl-object-case a
+                  :g-map (stobj-let ((logicman (interp-st->logicman interp-st)))
+                                    (ok val logicman)
+                                    (b* ((bfrstate (logicman->bfrstate))
+                                         ((unless (bfrstate-mode-is :aignet))
+                                          (mv nil nil logicman))
+                                         ((mv err varmap) (gl-object-alist-to-varmap a.alist bfrstate nil))
+                                         ((when err)
+                                          (cw "~x0 primitive error: ~@1" 'acl2::aig-eval-list err)
+                                          (mv nil nil logicman)))
+                                      (stobj-let ((aignet (logicman->aignet logicman))
+                                                  (strash (logicman->strash logicman)))
+                                                 (lits aignet strash)
+                                                 (b* (((mv lits xmemo strash aignet)
+                                                       (aignet::aiglist-to-aignet
+                                                        x.val nil varmap (aignet::default-gatesimp)
+                                                        strash aignet)))
+                                                   (fast-alist-free xmemo)
+                                                   (mv lits aignet strash))
+                                                 (b* ((bfrstate (logicman->bfrstate)))
+                                                   (mv t
+                                                       (aignet-lit-list->bools lits bfrstate)
+                                                       logicman))))
+                                    (mv ok val interp-st))
+                  :otherwise (mv nil nil interp-st))
+    :otherwise (mv nil nil interp-st))
+  :formula-check aig-eval-formula-checks)
+
+
