books/centaur/fgl/fancy-ev.lisp
@@ -31,20 +31,33 @@
 (in-package "FGL")
 
 (include-book "interp-st-bfrs-ok")
-
+(include-book "std/strings/decimal" :dir :system)
 (set-state-ok t)
 
+(defconst *logically-relevant-interp-st-fields*
+  '(:stack :logicman :bvar-db :pathcond :constraint :constraint-db
+    :equiv-contexts :reclimit :errmsg))
+
 (encapsulate
-  (((fancy-ev-primitive * * interp-st state) => (mv * *)
+  (((fancy-ev-primitive * * interp-st state) => (mv * * interp-st)
     :formals (fn args interp-st state)
     :guard (and (pseudo-fnsym-p fn)
                 (true-listp args)
                 (interp-st-bfrs-ok interp-st))))
   (local (defun fancy-ev-primitive (fn args interp-st state)
            (declare (xargs :stobjs (interp-st state))
-                    (ignore fn args interp-st state))
-           (mv nil nil))))
-    
+                    (ignore fn args state))
+           (mv nil nil interp-st)))
+
+  (defthm interp-st-get-of-fancy-ev-primitive
+    (implies (member (interp-st-field-fix key)
+                     *logically-relevant-interp-st-fields*)
+             (equal (interp-st-get key (mv-nth 2 (fancy-ev-primitive fn args interp-st state)))
+                    (interp-st-get key interp-st))))
+
+  (defthm interp-st-bfrs-ok-of-fancy-ev-primitive
+    (implies (interp-st-bfrs-ok interp-st)
+             (interp-st-bfrs-ok (mv-nth 2 (fancy-ev-primitive fn args interp-st state))))))
    
 (define fancy-ev-definition ((fn pseudo-fnsym-p) state)
   :returns (mv ok
@@ -64,6 +77,7 @@
         (mv nil nil nil)))
     (mv t formals body)))
 
+(set-state-ok t)
 
 (defines fancy-ev
   (define fancy-ev ((x pseudo-termp)
@@ -75,35 +89,36 @@
                     aokp)
     :well-founded-relation acl2::nat-list-<
     :measure (list reclimit (pseudo-term-count x))
-    :returns (mv errmsg val)
+    :returns (mv errmsg val new-interp-st)
     :verify-guards nil
     (pseudo-term-case x
-      :const (mv nil x.val)
-      :var (mv nil (cdr (hons-assoc-equal x.name alist)))
-      :lambda (b* (((mv err args)
+      :const (mv nil x.val interp-st)
+      :var (mv nil (cdr (hons-assoc-equal x.name alist)) interp-st)
+      :lambda (b* (((mv err args interp-st)
                     (fancy-ev-list x.args alist reclimit interp-st state hard-errp aokp))
-                   ((when err) (mv err nil)))
+                   ((when err) (mv err nil interp-st)))
                 (fancy-ev x.body
                           (pairlis$ x.formals args)
                           reclimit interp-st state hard-errp aokp))
       :fncall (b* (((when (and** (eq x.fn 'if) (eql (len x.args) 3)))
-                    (b* (((mv err test) (fancy-ev (first x.args) alist reclimit interp-st state hard-errp aokp))
-                         ((when err) (mv err nil)))
+                    (b* (((mv err test interp-st) (fancy-ev (first x.args) alist reclimit interp-st state hard-errp aokp))
+                         ((when err) (mv err nil interp-st)))
                       (if test
                           (fancy-ev (second x.args) alist reclimit interp-st state hard-errp aokp)
                         (fancy-ev (third x.args) alist reclimit interp-st state hard-errp aokp))))
                    ((when (and** (eq x.fn 'return-last) (eql (len x.args) 3)))
                     (b* ((arg1 (first x.args)))
-                      (prog2$
-                       (pseudo-term-case arg1
-                         :const (and (eq arg1.val 'progn)
-                                     (b* (((mv ?err ?arg1)
-                                           (fancy-ev (second x.args) alist reclimit interp-st state hard-errp aokp)))
-                                       nil))
-                         :otherwise nil)
-                       (fancy-ev (third x.args) alist reclimit interp-st state hard-errp aokp))))
-                   ((mv err args) (fancy-ev-list x.args alist reclimit interp-st state hard-errp aokp))
-                   ((when err) (mv err nil)))
+                      (b* ((interp-st
+                            (pseudo-term-case arg1
+                              :const (if (eq arg1.val 'progn)
+                                         (b* (((mv ?err ?arg1 interp-st)
+                                               (fancy-ev (second x.args) alist reclimit interp-st state hard-errp aokp)))
+                                           interp-st)
+                                       interp-st)
+                              :otherwise interp-st)))
+                        (fancy-ev (third x.args) alist reclimit interp-st state hard-errp aokp))))
+                   ((mv err args interp-st) (fancy-ev-list x.args alist reclimit interp-st state hard-errp aokp))
+                   ((when err) (mv err nil interp-st)))
                 (fancy-ev-fncall x.fn args reclimit interp-st state hard-errp aokp))))
 
   (define fancy-ev-fncall ((fn pseudo-fnsym-p)
@@ -112,25 +127,25 @@
                            (interp-st interp-st-bfrs-ok)
                            state hard-errp aokp)
     :measure (list reclimit 0)
-    :returns (mv errmsg val)
+    :returns (mv errmsg val new-interp-st)
     (b* ((fn (pseudo-fnsym-fix fn))
          (args (mbe :logic (true-list-fix args)
                     :exec args))
-         ((mv ev-ok val)
+         ((mv ev-ok val interp-st)
           (fancy-ev-primitive fn args interp-st state))
-         ((when ev-ok) (mv nil val))
+         ((when ev-ok) (mv nil val interp-st))
          ((mv ev-err val)
           (acl2::magic-ev-fncall fn
                                  args
                                  state hard-errp aokp))
-         ((unless ev-err) (mv nil val))
+         ((unless ev-err) (mv nil val interp-st))
          ((when (zp reclimit))
-          (mv (msg "Recursion limit ran out calling ~x0" (pseudo-fnsym-fix fn)) nil))
+          (mv (msg "Recursion limit ran out calling ~x0" (pseudo-fnsym-fix fn)) nil interp-st))
          ((mv def-ok formals body) (fancy-ev-definition fn state))
          ((unless def-ok)
-          (mv (msg "No definition for ~x0" (pseudo-fnsym-fix fn)) nil))
+          (mv (msg "No definition for ~x0" (pseudo-fnsym-fix fn)) nil interp-st))
          ((unless (eql (len formals) (len args)))
-          (mv (msg "Wrong arity for ~x0 call" (pseudo-fnsym-fix fn)) nil)))
+          (mv (msg "Wrong arity for ~x0 call" (pseudo-fnsym-fix fn)) nil interp-st)))
       (fancy-ev body (pairlis$ formals args) (1- reclimit) interp-st state hard-errp aokp)))
 
   (define fancy-ev-list ((x pseudo-term-listp)
@@ -139,16 +154,60 @@
                          (interp-st interp-st-bfrs-ok)
                          state hard-errp aokp)
     :measure (list reclimit (pseudo-term-list-count x))
-    :returns (mv errmsg (vals true-listp))
+    :returns (mv errmsg (vals true-listp) new-interp-st)
     (b* (((when (atom x))
-          (mv nil nil))
-         ((mv err first) (fancy-ev (car x) alist reclimit interp-st state hard-errp aokp))
-         ((when err) (mv err nil))
-         ((mv err rest) (fancy-ev-list (cdr x) alist reclimit interp-st state hard-errp aokp))
-         ((when err) (mv err nil)))
-      (mv nil (cons first rest))))
+          (mv nil nil interp-st))
+         ((mv err first interp-st) (fancy-ev (car x) alist reclimit interp-st state hard-errp aokp))
+         ((when err) (mv err nil interp-st))
+         ((mv err rest interp-st) (fancy-ev-list (cdr x) alist reclimit interp-st state hard-errp aokp))
+         ((when err) (mv err nil interp-st)))
+      (mv nil (cons first rest) interp-st)))
   ///
-  (verify-guards fancy-ev)
+  (local (in-theory (disable acl2::member-of-cons member (tau-system) pseudo-termp pseudo-term-listp
+                             fancy-ev fancy-ev-fncall fancy-ev-list)))
+  (defret-mutual interp-st-get-of-fancy-ev
+    (defret interp-st-get-of-<fn>
+      (implies (member (interp-st-field-fix key) *logically-relevant-interp-st-fields*)
+               (equal (interp-st-get key new-interp-st)
+                      (interp-st-get key interp-st)))
+      :hints ('(:expand (<call>)))
+      :fn fancy-ev)
+    (defret interp-st-get-of-<fn>
+      (implies (member (interp-st-field-fix key) *logically-relevant-interp-st-fields*)
+               (equal (interp-st-get key new-interp-st)
+                      (interp-st-get key interp-st)))
+      :hints ('(:expand (<call>)))
+      :fn fancy-ev-fncall)
+    (defret interp-st-get-of-<fn>
+      (implies (member (interp-st-field-fix key) *logically-relevant-interp-st-fields*)
+               (equal (interp-st-get key new-interp-st)
+                      (interp-st-get key interp-st)))
+      :hints ('(:expand (<call>)))
+      :fn fancy-ev-list))
+
+  (defret-mutual interp-st-bfrs-ok-of-fancy-ev
+    (defret interp-st-bfrs-ok-of-<fn>
+      (implies (interp-st-bfrs-ok interp-st)
+               (interp-st-bfrs-ok new-interp-st))
+      :hints ('(:expand (<call>)))
+      :fn fancy-ev)
+    (defret interp-st-bfrs-ok-of-<fn>
+      (implies (interp-st-bfrs-ok interp-st)
+               (interp-st-bfrs-ok new-interp-st))
+      :hints ('(:expand (<call>)))
+      :fn fancy-ev-fncall)
+    (defret interp-st-bfrs-ok-of-<fn>
+      (implies (interp-st-bfrs-ok interp-st)
+               (interp-st-bfrs-ok new-interp-st))
+      :hints ('(:expand (<call>)))
+      :fn fancy-ev-list))
+
+  (local (defthm true-listp-when-symbol-listp
+           (implies (symbol-listp x)
+                    (true-listp x))))
+
+  (verify-guards fancy-ev
+    :hints(("Goal" :in-theory (enable acl2::member-of-cons))))
 
   (local (in-theory (disable fancy-ev fancy-ev-list fancy-ev-fncall
                              pseudo-term-listp pseudo-termp)))
@@ -157,7 +216,7 @@
 
 
 
-
+(program)
 
 (defmacro fancy-ev-add-primitive (fn guard)
   `(table fancy-ev-primitives ',fn ',guard))
@@ -176,6 +235,19 @@
     (cons (or (car stobjs-in) (car formals))
           (fancy-ev-primitive-formals (cdr stobjs-in) (cdr formals)))))
 
+(defun fancy-ev-stobj-out-bindings (stobjs-out n)
+  (if (atom stobjs-out)
+      nil
+    (cons (or (car stobjs-out)
+              (intern-in-package-of-symbol (concatenate 'string "OUT" (str::natstr n)) 'fgl-fgl))
+          (fancy-ev-stobj-out-bindings (cdr stobjs-out) (+ 1 n)))))
+
+(defun fancy-ev-stobj-out-results (stobjs-out vars)
+  (if (atom stobjs-out)
+      nil
+    (cons (if (car stobjs-out) nil (car vars))
+          (fancy-ev-stobj-out-results (cdr stobjs-out) (cdr vars)))))
+
 (defun fancy-ev-primitives-cases (argsvar table state)
   (b* (((when (atom table)) nil)
        ((cons fn guard) (car table))
@@ -187,20 +259,34 @@
         (er hard? 'def-fancy-ev-primitives "~x0 takes input stobjs ~x1 -- only interp-st and state are allowed"
             fn diff))
        (stobjs-out (stobjs-out fn wrld))
-       (diff (set-difference-eq stobjs-out '(nil)))
+       (diff (set-difference-eq stobjs-out '(nil interp-st)))
        ((when diff)
-        (er hard? 'def-fancy-ev-primitives "~x0 can modify stobjs ~x1 -- no stobj modification is allowed"
+        (er hard? 'def-fancy-ev-primitives "~x0 can modify stobjs ~x1 -- only interp-st may be modified"
             fn diff))
        (bindings (fancy-ev-primitive-bindings argsvar stobjs-in formals 0))
-       (call-formals (fancy-ev-primitive-formals stobjs-in formals)))
-    `((,fn (mv t (b* ,bindings
-                   (mbe :logic (non-exec (,fn . ,call-formals))
-                        :exec (if ,guard
-                                  ,(if (consp (cdr stobjs-out))
-                                       `(mv-list ,(len stobjs-out)
-                                                 (,fn . ,call-formals))
-                                     `(,fn . ,call-formals))
-                                (non-exec (ec-call (,fn . ,call-formals))))))))
+       (call-formals (fancy-ev-primitive-formals stobjs-in formals))
+       ((unless (member 'interp-st stobjs-out))
+        `((,fn (b* (,@bindings
+                    (result (mbe :logic (non-exec (,fn . ,call-formals))
+                                 :exec (if ,guard
+                                           ,(if (consp (cdr stobjs-out))
+                                                `(mv-list ,(len stobjs-out)
+                                                          (,fn . ,call-formals))
+                                              `(,fn . ,call-formals))
+                                         (non-exec (ec-call (,fn . ,call-formals)))))))
+                 (mv t result interp-st)))
+          . ,(fancy-ev-primitives-cases argsvar (cdr table) state)))
+       (out-bindings (fancy-ev-stobj-out-bindings stobjs-out 0))
+       (results (fancy-ev-stobj-out-results stobjs-out out-bindings)))
+    `((,fn (b* (,@bindings
+                (,@(if (consp (cdr stobjs-out))
+                       `((mv . ,out-bindings))
+                     out-bindings)
+                 (mbe :logic (,fn . ,call-formals)
+                      :exec (if ,guard
+                                (,fn . ,call-formals)
+                              (ec-call (,fn . ,call-formals))))))
+             (mv t (list . ,results) interp-st)))
       . ,(fancy-ev-primitives-cases argsvar (cdr table) state))))
 
 
@@ -210,12 +296,20 @@
                       (args true-listp)
                       (interp-st interp-st-bfrs-ok)
                       state)
+       :ignore-ok t
+       :irrelevant-formals-ok t
        (case (pseudo-fnsym-fix fn)
          ,@(fancy-ev-primitives-cases 'args prims state)
-         (otherwise (mv nil nil)))
+         (otherwise (mv nil nil interp-st)))
        ///
        (defattach fancy-ev-primitive ,fnname))))
 
 (defmacro def-fancy-ev-primitives (fnname)
   `(make-event
     (def-fancy-ev-primitives-fn ',fnname state)))
+
+;; (logic)
+
+;; (fancy-ev-add-primitive update-interp-st->cgraph$inline (cgraph-p cgraph))
+
+;; (def-fancy-ev-primitives foo-bar)
