books/centaur/fgl/top.lisp
@@ -32,158 +32,58 @@
 
 (include-book "clauseproc")
 (include-book "def-gl-rewrite")
-(include-book "subst-functions")
+;; (include-book "subst-functions")
 (include-book "primitives")
 (include-book "fgarrays")
+(include-book "aig-eval")
 (include-book "sat")
 (include-book "ctrex-utils")
 
-(program)
+;; ----------------------------------------------------------------------
+;; Install GL primitives:  This event collects the primitives defined in
+;; primitives, fgarrays, and fast-alists and defines a new function
+;; top-primitive-fncall, which is attached to gl-primitive-fncall-stub.
+;; This event may be repeated later (with a different prefix instead of top)
+;; to install more primitives.
 
-(defun attachment-pairs (fns wrld)
-  (b* (((when (atom fns)) nil)
-       (fn (car fns))
-       (pair (acl2::attachment-pair fn wrld))
-       ((unless (consp pair))
-        (attachment-pairs (cdr fns) wrld)))
-    (cons pair (attachment-pairs (cdr fns) wrld))))
-
-(defun attachment-pairs! (fns wrld)
-  (b* (((when (atom fns)) nil)
-       (fn (car fns))
-       (pair (acl2::attachment-pair fn wrld))
-       ((unless (consp pair))
-        (er hard? 'attachment-pairs!
-            "Function ~x0 is required to have an attachment.")))
-    (cons pair (attachment-pairs! (cdr fns) wrld))))
-    
-
-(defun gl-clause-proc-define-subst-functions (prefix constname wrld)
-  (b* ((pairs (append (attachment-pairs '(fgl-ev
-                                          fgl-ev-list
-                                          fgl-ev-meta-extract-global-badguy
-                                          fgl-ev-falsify
-                                          fgl-apply
-                                          fgl-object-eval-fn
-                                          fgl-objectlist-eval-fn
-                                          fgl-object-alist-eval-fn)
-                                        wrld)
-                      (attachment-pairs! '(gl-primitive-fncall-stub
-                                           gl-primitive-formula-checks-stub) wrld)))
-       ((mv event subst)
-        (substitute-functions
-         prefix '(gl-interp-cp) pairs wrld)))
-    `(progn ,event
-            (defconst ,constname ',subst))))
+(install-gl-primitives top)
 
 
-(defun gl-clause-proc-correctness-thm (prefix subst)
-  `(defthm ,(intern-in-package-of-symbol
-             (concatenate 'string (symbol-name prefix) "-GL-INTERP-CP-CORRECT")
-             prefix)
-     ,(sublis (pairlis$ (strip-cars subst)
-                        (acl2::strip-cadrs subst))
-              '(implies (and (pseudo-term-listp clause)
-                             (alistp a)
-                             (fgl-ev
-                              (meta-extract-global-fact+
-                               (mv-nth 0 (fgl-ev-meta-extract-global-badguy state))
-                               (mv-nth 1 (fgl-ev-meta-extract-global-badguy state))
-                               state)
-                              (fgl-ev-falsify
-                               (meta-extract-global-fact+
-                                (mv-nth 0 (fgl-ev-meta-extract-global-badguy state))
-                                (mv-nth 1 (fgl-ev-meta-extract-global-badguy state))
-                                state)))
-                             (fgl-ev (conjoin-clauses
-                                      (acl2::clauses-result (gl-interp-cp clause hint state)))
-                                     a))
-                        (fgl-ev (disjoin clause) a)))
-     :hints (("goal" :by (:functional-instance gl-interp-cp-correct1
-                          . ,subst)
-              :do-not '(preprocess simplify)))
-     :rule-classes :clause-processor))
+
+;; ----------------------------------------------------------------------
+;; Def-fancy-ev-primitives.  This event collects the functions that are stored
+;; in the fancy-ev-primitives table (added by fancy-ev-add-primitive) and
+;; installs them in a new function that is attached to fancy-ev-primitive.
+;; These functions can then be used in syntax-bind forms.  (They could be used
+;; in syntaxp/bind-free forms as well, but at the moment those won't be
+;; translated if interp-st is used.)
+(fancy-ev-add-primitive interp-st-prev-bindings
+                        (< 1 (interp-st-stack-frames interp-st)))
+
+(fancy-ev-add-primitive interp-st-ipasir-counterex-stack-prev-bindings/print-errors
+                        (< 1 (interp-st-stack-frames interp-st)))
+
+(fancy-ev-add-primitive interp-st-ipasir-counterex-bindings/print-errors
+                        (and (gl-object-bindings-p x)
+                             (interp-st-bfr-listp (gl-object-bindings-bfrlist x))))
+
+(fancy-ev-add-primitive interp-st-ipasir-counterex-stack-bindings/print-errors t)
+
+(fancy-ev-add-primitive interp-st-ipasir-counterex-bindings
+                        (and (gl-object-bindings-p x)
+                             (interp-st-bfr-listp (gl-object-bindings-bfrlist x))))
+
+(fancy-ev-add-primitive interp-st-ipasir-counterex-stack-bindings t)
+
+(fancy-ev-add-primitive get-global (and (symbolp x)
+                                        (boundp-global x state)))
+
+(def-fancy-ev-primitives counterex-primitives)
 
 
-(defun def-gl-clause-proc-fn (name wrld)
-  (declare (xargs :mode :program)
-           (ignore wrld))
-  (b* (((unless (str::strsuffixp "-GL-INTERP-CP" (symbol-name name)))
-        (er hard? 'def-gl-clause-proc-fn "Name must end in -GL-INTERP-CP"))
-       (prefix (intern-in-package-of-symbol
-                (subseq (symbol-name name) 0 (- (length (symbol-name name))
-                                                (length "-GL-INTERP-CP")))
-                name))
-       (prefix- (intern-in-package-of-symbol
-                 (concatenate 'string (symbol-name prefix) "-")
-                 name))
-       (constname (intern-in-package-of-symbol
-                   (concatenate 'string "*" (symbol-name name) "-SUBST*")
-                   name))
-       ;; (default-hints (default-hints wrld))
-       ;; (pairs (append (attachment-pairs '(fgl-ev
-       ;;                                    fgl-ev-list
-       ;;                                    fgl-ev-meta-extract-global-badguy
-       ;;                                    fgl-ev-falsify
-       ;;                                    fgl-apply
-       ;;                                    fgl-object-eval
-       ;;                                    fgl-objectlist-eval)
-       ;;                                  wrld)
-       ;;                (attachment-pairs! '(gl-primitive-fncall-stub) wrld)))
-       ;; ((mv event subst)
-       ;;  (substitute-functions
-       ;;   prefix
-       ;;   '(gl-interp-cp)
-       ;;   pairs
-       ;;   wrld))
-       )
-    `(with-output :off :all :on (error summary) :gag-mode nil
-       (progn
-         (install-gl-primitives ,prefix)
-         (make-event
-          (acl2::template-subst
-           '(set-default-hints
-             '((let ((term (car (last clause))))
-                 (case-match term
-                   (('equal (fn . args) . &)
-                    (cond ((or (member fn '(<prefix>-ev
-                                            <prefix>-ev-list))
-                               (not (symbol-listp args)))
-                           '(:do-not nil :in-theory (enable)))
-                          ;; ((member fn '(<prefix>-ev-falsify
-                          ;;               <prefix>-meta-extract-global-badguy))
-                          ;;  `(:by 
-                          (t `(:clause-processor (beta-reduce-by-hint-cp clause ',fn state)
-                               :do-not nil :in-theory (enable)))))
-                   (& (cond ((member-atoms '<prefix>-primitive-fncall term)
-                             '(:do-not nil :in-theory (enable)))
-                            ((member-atoms '<prefix>-ev-meta-extract-global-badguy term)
-                             '(:by <prefix>-ev-meta-extract-global-badguy))
-                            ((member-atoms '<prefix>-ev-falsify term)
-                             `(:clause-processor (beta-reduce-by-hint-cp clause '<prefix>-ev-falsify state)
-                               :do-not nil :in-theory (enable)))
-                            (t '(:do-not nil
-                                 :in-theory (enable <prefix>-ev-of-fncall-args
-                                                    <prefix>-ev-of-nonsymbol-atom
-                                                    <prefix>-ev-of-bad-fncall)))))))))
-           :str-alist `(("<PREFIX>" ,,(symbol-name prefix) . ,',prefix))))
-         (make-event
-          (gl-clause-proc-define-subst-functions ',prefix- ',constname (w state)))
-         
-         (make-event
-          (gl-clause-proc-correctness-thm ',prefix ,constname))))))
-
-(defmacro def-gl-clause-proc (name)
-  `(make-event
-    (def-gl-clause-proc-fn ',name (w state))))
-
-(logic)
-(set-ignore-ok t)
-(set-irrelevant-formals-ok t)
-
-(set-case-split-limitations '(0 1000))
-(def-gl-clause-proc top-gl-interp-cp)
-
+;; Convenience macro to create a glcp-config object that captures the current
+;; definitions, rewrite rules, branch merge rules, and function modes from
+;; their respective tables.
 (defmacro default-glcp-config ()
   '(make-glcp-config
     :rewrite-rule-table (table-alist 'gl-rewrite-rules (w state))
